eve/Src/framework/eiffel2boogie/translation/pool/e2b_tu_frame.e
@@ -28,7 +28,7 @@ feature -- Basic operations
 			l_translator: E2B_ROUTINE_TRANSLATOR
 		do
 			create l_translator.make
-			l_translator.translate_writes_function (feat, type)
+			l_translator.translate_frame_function (feat, type)
 		end
 
 end
